correctness/RegexCorrectness/Data/Expr/Semantics/Separation.lean
@@ -5,14 +5,14 @@ import RegexCorrectness.Data.Expr.Semantics.Captures
 namespace Regex.Data.Expr
 
 def tags : Expr → Finset Nat
-| .empty | .epsilon | .char _ | .classes _ => ∅
+| .empty | .epsilon | .anchor _ | .char _ | .classes _ => ∅
 | .group tag e => {tag} ∪ e.tags
 | .alternate e₁ e₂ => e₁.tags ∪ e₂.tags
 | .concat e₁ e₂ => e₁.tags ∪ e₂.tags
 | .star e => e.tags
 
 def Disjoint : Expr → Prop
-| .empty | .epsilon | .char _ | .classes _ => True
+| .empty | .epsilon | .anchor _ | .char _ | .classes _ => True
 | .group tag e => tag ∉ e.tags ∧ e.Disjoint
 | .alternate e₁ e₂ => e₁.tags ∩ e₂.tags = ∅ ∧ e₁.Disjoint ∧ e₂.Disjoint
 | .concat e₁ e₂ => e₁.tags ∩ e₂.tags = ∅ ∧ e₁.Disjoint ∧ e₂.Disjoint
