correctness/RegexCorrectness/VM/EpsilonClosure/Basic.lean
@@ -34,6 +34,12 @@ def εClosure' (nfa : NFA) (wf : nfa.WellFormed) (it : Iterator)
       | .epsilon state' =>
         have isLt : state' < nfa.nodes.size := wf.inBounds' state hn
         εClosure' nfa wf it matched ⟨states', next.updates⟩ ((update, ⟨state', isLt⟩) :: stack')
+      | .anchor anchor state' =>
+        have isLt : state' < nfa.nodes.size := wf.inBounds' state hn
+        if anchor.test it then
+          εClosure' nfa wf it matched ⟨states', next.updates⟩ ((update, ⟨state', isLt⟩) :: stack')
+        else
+          εClosure' nfa wf it matched ⟨states', next.updates⟩ stack'
       | .split state₁ state₂ =>
         have isLt : state₁ < nfa.nodes.size ∧ state₂ < nfa.nodes.size := wf.inBounds' state hn
         εClosure' nfa wf it matched ⟨states', next.updates⟩ ((update, ⟨state₁, isLt.1⟩) :: (update, ⟨state₂, isLt.2⟩):: stack')
@@ -54,68 +60,189 @@ def εClosure' (nfa : NFA) (wf : nfa.WellFormed) (it : Iterator)
       | .fail => εClosure' nfa wf it matched ⟨states', next.updates⟩ stack'
 termination_by (next.states.measure, stack)
 
+#check εClosure'.induct
+
+/-
+Regex.VM.εClosure'.induct (nfa : NFA) (wf : nfa.WellFormed) (it : Iterator)
+  (motive : Option (List (ℕ × Pos)) → SearchState' nfa → εStack' nfa → Prop)
+  (case1 : ∀ (matched : Option (List (ℕ × Pos))) (next : SearchState' nfa), motive matched next [])
+  (case2 :
+    ∀ (matched : Option (List (ℕ × Pos))) (next : SearchState' nfa) (update : List (ℕ × Pos))
+      (state : Fin nfa.nodes.size) (stack' : List (List (ℕ × Pos) × Fin nfa.nodes.size)),
+      state ∈ next.states → motive matched next stack' → motive matched next ((update, state) :: stack'))
+  (case3 :
+    ∀ (matched : Option (List (ℕ × Pos))) (next : SearchState' nfa) (update : List (ℕ × Pos))
+      (state : Fin nfa.nodes.size) (stack' : List (List (ℕ × Pos) × Fin nfa.nodes.size)),
+      state ∉ next.states →
+        let states' := next.states.insert state;
+        ∀ (state' : ℕ),
+          nfa[state] = NFA.Node.epsilon state' →
+            ∀ (isLt : state' < nfa.nodes.size),
+              motive matched { states := states', updates := next.updates } ((update, ⟨state', isLt⟩) :: stack') →
+                motive matched next ((update, state) :: stack'))
+  (case4 :
+    ∀ (matched : Option (List (ℕ × Pos))) (next : SearchState' nfa) (update : List (ℕ × Pos))
+      (state : Fin nfa.nodes.size) (stack' : List (List (ℕ × Pos) × Fin nfa.nodes.size)),
+      state ∉ next.states →
+        let states' := next.states.insert state;
+        ∀ (anchor : Data.Anchor) (state' : ℕ),
+          nfa[state] = NFA.Node.anchor anchor state' →
+            ∀ (isLt : state' < nfa.nodes.size),
+              Data.Anchor.test it anchor = true →
+                motive matched { states := states', updates := next.updates } ((update, ⟨state', isLt⟩) :: stack') →
+                  motive matched next ((update, state) :: stack'))
+  (case5 :
+    ∀ (matched : Option (List (ℕ × Pos))) (next : SearchState' nfa) (update : List (ℕ × Pos))
+      (state : Fin nfa.nodes.size) (stack' : List (List (ℕ × Pos) × Fin nfa.nodes.size)),
+      state ∉ next.states →
+        let states' := next.states.insert state;
+        ∀ (anchor : Data.Anchor) (state' : ℕ),
+          nfa[state] = NFA.Node.anchor anchor state' →
+            state' < nfa.nodes.size →
+              ¬Data.Anchor.test it anchor = true →
+                motive matched { states := states', updates := next.updates } stack' →
+                  motive matched next ((update, state) :: stack'))
+  (case6 :
+    ∀ (matched : Option (List (ℕ × Pos))) (next : SearchState' nfa) (update : List (ℕ × Pos))
+      (state : Fin nfa.nodes.size) (stack' : List (List (ℕ × Pos) × Fin nfa.nodes.size)),
+      state ∉ next.states →
+        let states' := next.states.insert state;
+        ∀ (state₁ state₂ : ℕ),
+          nfa[state] = NFA.Node.split state₁ state₂ →
+            ∀ (isLt : state₁ < nfa.nodes.size ∧ state₂ < nfa.nodes.size),
+              motive matched { states := states', updates := next.updates }
+                  ((update, ⟨state₁, ⋯⟩) :: (update, ⟨state₂, ⋯⟩) :: stack') →
+                motive matched next ((update, state) :: stack'))
+  (case7 :
+    ∀ (matched : Option (List (ℕ × Pos))) (next : SearchState' nfa) (update : List (ℕ × Pos))
+      (state : Fin nfa.nodes.size) (stack' : List (List (ℕ × Pos) × Fin nfa.nodes.size)),
+      state ∉ next.states →
+        let states' := next.states.insert state;
+        ∀ (offset state' : ℕ),
+          nfa[state] = NFA.Node.save offset state' →
+            ∀ (isLt : state' < nfa.nodes.size),
+              let update' := update ++ [(offset, it.pos)];
+              motive matched { states := states', updates := next.updates } ((update', ⟨state', isLt⟩) :: stack') →
+                motive matched next ((update, state) :: stack'))
+  (case8 :
+    ∀ (matched : Option (List (ℕ × Pos))) (next : SearchState' nfa) (update : List (ℕ × Pos))
+      (state : Fin nfa.nodes.size) (stack' : List (List (ℕ × Pos) × Fin nfa.nodes.size)),
+      state ∉ next.states →
+        let states' := next.states.insert state;
+        nfa[state] = NFA.Node.done →
+          let matched' := matched <|> some update;
+          let updates' := next.updates.set (↑state) update ⋯;
+          motive matched' { states := states', updates := updates' } stack' →
+            motive matched next ((update, state) :: stack'))
+  (case9 :
+    ∀ (matched : Option (List (ℕ × Pos))) (next : SearchState' nfa) (update : List (ℕ × Pos))
+      (state : Fin nfa.nodes.size) (stack' : List (List (ℕ × Pos) × Fin nfa.nodes.size)),
+      state ∉ next.states →
+        let states' := next.states.insert state;
+        ∀ (c : Char) (state' : ℕ),
+          nfa[state] = NFA.Node.char c state' →
+            let updates' := next.updates.set (↑state) update ⋯;
+            motive matched { states := states', updates := updates' } stack' →
+              motive matched next ((update, state) :: stack'))
+  (case10 :
+    ∀ (matched : Option (List (ℕ × Pos))) (next : SearchState' nfa) (update : List (ℕ × Pos))
+      (state : Fin nfa.nodes.size) (stack' : List (List (ℕ × Pos) × Fin nfa.nodes.size)),
+      state ∉ next.states →
+        let states' := next.states.insert state;
+        ∀ (cs : Data.Classes) (state' : ℕ),
+          nfa[state] = NFA.Node.sparse cs state' →
+            let updates' := next.updates.set (↑state) update ⋯;
+            motive matched { states := states', updates := updates' } stack' →
+              motive matched next ((update, state) :: stack'))
+  (case11 :
+    ∀ (matched : Option (List (ℕ × Pos))) (next : SearchState' nfa) (update : List (ℕ × Pos))
+      (state : Fin nfa.nodes.size) (stack' : List (List (ℕ × Pos) × Fin nfa.nodes.size)),
+      state ∉ next.states →
+        let states' := next.states.insert state;
+        nfa[state] = NFA.Node.fail →
+          motive matched { states := states', updates := next.updates } stack' →
+            motive matched next ((update, state) :: stack'))
+  (matched : Option (List (ℕ × Pos))) (next : SearchState' nfa) (stack : εStack' nfa) : motive matched next stack
+-/
+
 -- Cleaner version of the fuction induction principle
 -- Using tactics in the body crashes Lean due to too high memory usage
-theorem εClosure'.induct' (nfa : NFA) (wf : nfa.WellFormed) (it : Iterator)
-  (motive : Option (List (Nat × Pos)) → SearchState' nfa → εStack' nfa → Prop)
-  (base : ∀ matched next, motive matched next [])
-  (visited :
-    ∀ matched next update state stack',
-    state ∈ next.states →
-    motive matched next stack' →
-    motive matched next ((update, state) :: stack'))
-  (epsilon : ∀ matched next update state stack' state',
-    state ∉ next.states → nfa[state] = .epsilon state' →
-    let next' := ⟨next.states.insert state, next.updates⟩;
-    motive matched next' ((update, state') :: stack') →
-    motive matched next ((update, state) :: stack'))
-  (split : ∀ matched next update state stack' state₁ state₂,
-    state ∉ next.states → nfa[state] = .split state₁ state₂ →
-    let next' := ⟨next.states.insert state, next.updates⟩;
-    motive matched next' ((update, state₁) :: (update, state₂) :: stack') →
-    motive matched next ((update, state) :: stack'))
-  (save : ∀ matched next update state stack' offset state',
-    state ∉ next.states → nfa[state] = .save offset state' →
-    let next' := ⟨next.states.insert state, next.updates⟩;
-    motive matched next' ((update ++ [(offset, it.pos)], state') :: stack') →
-    motive matched next ((update, state) :: stack'))
-  (done : ∀ matched next update state stack',
-    state ∉ next.states → nfa[state] = .done →
-    let next' := ⟨next.states.insert state, next.updates.set state update⟩;
-    motive (matched <|> .some update) next' stack' →
-    motive matched next ((update, state) :: stack'))
-  (char : ∀ matched next update state stack' c (state' : Fin nfa.nodes.size),
-    state ∉ next.states → nfa[state] = .char c state' →
-    let next' := ⟨next.states.insert state, next.updates.set state update⟩;
-    motive matched next' stack' →
-    motive matched next ((update, state) :: stack'))
-  (sparse : ∀ matched next update state stack' cs (state' : Fin nfa.nodes.size),
-    state ∉ next.states → nfa[state] = .sparse cs state' →
-    let next' := ⟨next.states.insert state, next.updates.set state update⟩;
-    motive matched next' stack' →
-    motive matched next ((update, state) :: stack'))
-  (fail : ∀ matched next update state stack',
-    state ∉ next.states → nfa[state] = .fail →
-    let next' := ⟨next.states.insert state, next.updates⟩;
-    motive matched next' stack' →
-    motive matched next ((update, state) :: stack')) :
-  ∀ matched next stack, motive matched next stack := fun matched next stack =>
-    εClosure'.induct nfa wf it motive base visited
-      (fun matched next update state stack' mem state' hn isLt ih =>
-        epsilon matched next update state stack' ⟨state', isLt⟩ mem hn ih)
-      (fun matched next update state stack' mem state₁ state₂ hn isLt ih =>
-        split matched next update state stack' ⟨state₁, isLt.1⟩ ⟨state₂, isLt.2⟩ mem hn ih)
-      (fun matched next update state stack' mem offset state' hn isLt ih =>
-        save matched next update state stack' offset ⟨state', isLt⟩ mem hn ih)
-      (fun matched next update state stack' mem hn ih =>
-        done matched next update state stack' mem hn ih)
-      (fun matched next update state stack' mem c state' hn ih =>
-        char matched next update state stack' c ⟨state', wf.inBounds' state hn⟩ mem hn ih)
-      (fun matched next update state stack' mem cs state' hn ih =>
-        sparse matched next update state stack' cs ⟨state', wf.inBounds' state hn⟩ mem hn ih)
-      (fun matched next update state stack' mem hn ih =>
-        fail matched next update state stack' mem hn ih)
-      matched next stack
+-- theorem εClosure'.induct' (nfa : NFA) (wf : nfa.WellFormed) (it : Iterator)
+--   (motive : Option (List (Nat × Pos)) → SearchState' nfa → εStack' nfa → Prop)
+--   (base : ∀ matched next, motive matched next [])
+--   (visited :
+--     ∀ matched next update state stack',
+--     state ∈ next.states →
+--     motive matched next stack' →
+--     motive matched next ((update, state) :: stack'))
+--   (epsilon : ∀ matched next update state stack' state',
+--     state ∉ next.states → nfa[state] = .epsilon state' →
+--     let next' := ⟨next.states.insert state, next.updates⟩;
+--     motive matched next' ((update, state') :: stack') →
+--     motive matched next ((update, state) :: stack'))
+--   (anchor_pos : ∀ matched next update state stack' anchor state',
+--     state ∉ next.states → nfa[state] = .anchor anchor state' →
+--     let next' := ⟨next.states.insert state, next.updates⟩;
+--     anchor.test it →
+--     motive matched next' ((update, state') :: stack') →
+--     motive matched next ((update, state) :: stack'))
+--   (anchor_neg : ∀ matched next update state stack' anchor state',
+--     state ∉ next.states → nfa[state] = .anchor anchor state' →
+--     let next' := ⟨next.states.insert state, next.updates⟩;
+--     ¬anchor.test it →
+--     motive matched next' stack' →
+--     motive matched next ((update, state) :: stack'))
+--   (split : ∀ matched next update state stack' state₁ state₂,
+--     state ∉ next.states → nfa[state] = .split state₁ state₂ →
+--     let next' := ⟨next.states.insert state, next.updates⟩;
+--     motive matched next' ((update, state₁) :: (update, state₂) :: stack') →
+--     motive matched next ((update, state) :: stack'))
+--   (save : ∀ matched next update state stack' offset state',
+--     state ∉ next.states → nfa[state] = .save offset state' →
+--     let next' := ⟨next.states.insert state, next.updates⟩;
+--     motive matched next' ((update ++ [(offset, it.pos)], state') :: stack') →
+--     motive matched next ((update, state) :: stack'))
+--   (done : ∀ matched next update state stack',
+--     state ∉ next.states → nfa[state] = .done →
+--     let next' := ⟨next.states.insert state, next.updates.set state update⟩;
+--     motive (matched <|> .some update) next' stack' →
+--     motive matched next ((update, state) :: stack'))
+--   (char : ∀ matched next update state stack' c (state' : Fin nfa.nodes.size),
+--     state ∉ next.states → nfa[state] = .char c state' →
+--     let next' := ⟨next.states.insert state, next.updates.set state update⟩;
+--     motive matched next' stack' →
+--     motive matched next ((update, state) :: stack'))
+--   (sparse : ∀ matched next update state stack' cs (state' : Fin nfa.nodes.size),
+--     state ∉ next.states → nfa[state] = .sparse cs state' →
+--     let next' := ⟨next.states.insert state, next.updates.set state update⟩;
+--     motive matched next' stack' →
+--     motive matched next ((update, state) :: stack'))
+--   (fail : ∀ matched next update state stack',
+--     state ∉ next.states → nfa[state] = .fail →
+--     let next' := ⟨next.states.insert state, next.updates⟩;
+--     motive matched next' stack' →
+--     motive matched next ((update, state) :: stack')) :
+--   ∀ matched next stack, motive matched next stack := fun matched next stack =>
+--     εClosure'.induct nfa wf it motive base visited
+--       (fun matched next update state stack' mem state' hn isLt ih =>
+--         epsilon matched next update state stack' ⟨state', isLt⟩ mem hn ih)
+--       (fun matched next update state stack' mem a state' hn isLt h ih =>
+--         anchor_pos matched next update state stack' a ⟨state', isLt⟩ mem hn h ih)
+--       (fun matched next update state stack' mem a state' hn isLt h ih =>
+--         anchor_neg matched next update state stack' a ⟨state', isLt⟩ mem hn h ih)
+--       (fun matched next update state stack' mem state₁ state₂ hn isLt ih =>
+--         split matched next update state stack' ⟨state₁, isLt.1⟩ ⟨state₂, isLt.2⟩ mem hn ih)
+--       (fun matched next update state stack' mem offset state' hn isLt ih =>
+--         save matched next update state stack' offset ⟨state', isLt⟩ mem hn ih)
+--       (fun matched next update state stack' mem hn ih =>
+--         done matched next update state stack' mem hn ih)
+--       (fun matched next update state stack' mem c state' hn ih =>
+--         char matched next update state stack' c ⟨state', wf.inBounds' state hn⟩ mem hn ih)
+--       (fun matched next update state stack' mem cs state' hn ih =>
+--         sparse matched next update state stack' cs ⟨state', wf.inBounds' state hn⟩ mem hn ih)
+--       (fun matched next update state stack' mem hn ih =>
+--         fail matched next update state stack' mem hn ih)
+--       matched next stack
 
 /-
 Simplification lemmas for `εClosure'`.
@@ -143,6 +270,26 @@ theorem εClosure'_epsilon {update state stack' state'} (hmem : state ∉ next.s
     unfold εClosure'
     simp [hmem]
   split <;> simp_all
+
+@[simp]
+theorem εClosure'_anchor_pos {update state stack' anchor state'} (hmem : state ∉ next.states) (hn : nfa[state] = .anchor anchor state') (h : anchor.test it) :
+  εClosure' nfa wf it matched next ((update, state) :: stack') =
+  εClosure' nfa wf it matched ⟨next.states.insert state, next.updates⟩ ((update, state') :: stack') := by
+  conv =>
+    lhs
+    unfold εClosure'
+    simp [hmem]
+  sorry
+
+@[simp]
+theorem εClosure'_anchor_neg {update state stack' anchor state'} (hmem : state ∉ next.states) (hn : nfa[state] = .anchor anchor state') (h : ¬anchor.test it) :
+  εClosure' nfa wf it matched next ((update, state) :: stack') =
+  εClosure' nfa wf it matched ⟨next.states.insert state, next.updates⟩ stack' := by
+  conv =>
+    lhs
+    unfold εClosure'
+    simp [hmem]
+  sorry
 
 @[simp]
 theorem εClosure'_split {update state stack' state₁ state₂} (hmem : state ∉ next.states) (hn : nfa[state] = .split state₁ state₂) :
